coq/LLVMGen/Utils.v
@@ -64,9 +64,6 @@ Definition string_of_Γ (Γ:list (ident * typ)) : string
                                   )
                            Γ) ++ "]".
 
-Definition Same_t e `{canonical_names.Equiv e} (B C : t e) := forall k : key, find (elt:=e) k B = find (elt:=e) k C.
-    (* Same Extensionality property as [Extensionality_Ensembles] in [Coq.Sets.Ensembles]. *)
-Axiom Extensionality_t : forall e `{canonical_names.Equiv e} (A B: t e), Same_t A B -> A = B.
 
 Lemma typ_to_dtyp_P :
     forall t s,
